wip: more progress

lang_ghost.v
@@ -1,6 +1,19 @@
 From iris_io Require Export lang.
 
-Fixpoint ghost_ok(e: expr): Prop :=
+Section Autosubst_Lemmas.
+  Context {term : Type} {Ids_term : Ids term}
+          {Rename_term : Rename term} {Subst_term : Subst term}
+          {SubstLemmas_term : SubstLemmas term}.
+
+  Lemma iter_up (m x : nat) (f : var → term) :
+    upn m f x = if lt_dec x m then ids x else rename (+m) (f (x - m)).
+  Proof.
+    revert x; induction m as [|m IH]=> -[|x];
+      repeat (case_match || asimpl || rewrite IH); auto with omega.
+  Qed.
+End Autosubst_Lemmas.
+
+Fixpoint ghost_ok (e: expr): Prop :=
   match e with
   | Var x => True
   | Unit => True
@@ -20,134 +33,159 @@ Fixpoint ghost_ok(e: expr): Prop :=
   | _ => False
   end.
 
-  Inductive var_erases_to: list bool -> var -> var -> Prop :=
-  | var_erases_to_real_O gs:
+Lemma ghost_ok_subst e f : (forall x, ghost_ok (f x)) → ghost_ok e → ghost_ok e.[f].
+Proof. revert f; induction e; intros f Hf; asimpl; intuition auto. Qed.
+
+
+Inductive var_erases_to: list bool -> var -> var -> Prop :=
+| var_erases_to_real_O gs:
     var_erases_to (false :: gs) O O
-  | var_erases_to_real_S gs x x':
+| var_erases_to_real_S gs x x':
     var_erases_to gs x x' ->
     var_erases_to (false :: gs) (S x) (S x')
-  | var_erases_to_ghost_S gs x x':
+| var_erases_to_ghost_S gs x x':
     var_erases_to gs x x' ->
-    var_erases_to (true :: gs) (S x) x'
-  .
+    var_erases_to (true :: gs) (S x) x'.
 
-  Inductive erases_to_core : list bool -> expr -> expr -> Prop :=
+Lemma var_erases_to_not_ghost gs x y :
+  var_erases_to gs x y → gs !! x = Some false.
+Proof. induction 1; auto. Qed.
+
+
+  Lemma var_erases_to_closed gb x x' f :
+    var_erases_to gb x x' → (Var x).[upn (length gb) f] = Var x.
+  Proof.
+    induction 1; asimpl in *; auto.
+    - by rewrite IHvar_erases_to.
+    - by rewrite IHvar_erases_to.
+  Qed.
+
+Inductive erases_to : nat → list bool -> expr -> expr -> Prop :=
   | Var_erases_to gs x x':
     var_erases_to gs x x' ->
-    erases_to_core gs (Var x) (Var x')
-  | Rec_erases_to gs e e':
-    erases_to (false :: false :: gs) e e' ->
-    erases_to_core gs (Rec e) (Rec e')
-  | Lam_erases_to gs e e':
-    erases_to (false :: gs) e e' ->
-    erases_to_core gs (Lam e) (Lam e')
-  | LetIn_erases_to gs e1 e2 e1' e2':
-    erases_to gs e1 e1' ->
-    erases_to (false :: gs) e2 e2' ->
-    erases_to_core gs (LetIn e1 e2) (LetIn e1' e2')
-  | Seq_erases_to gs e1 e2 e1' e2':
-    erases_to gs e1 e1' ->
-    erases_to gs e2 e2' ->
-    erases_to_core gs (Seq e1 e2) (Seq e1' e2')
-  | App_erases_to gs e1 e2 e1' e2':
-    erases_to gs e1 e1' ->
-    erases_to gs e2 e2' ->
-    erases_to_core gs (App e1 e2) (App e1' e2')
+    erases_to 0 gs (Var x) (Var x')
+  | Rec_erases_to n gs e e':
+    erases_to n (false :: false :: gs) e e' ->
+    erases_to (S n) gs (Rec e) (Rec e')
+  | Lam_erases_to n gs e e':
+    erases_to n (false :: gs) e e' ->
+    erases_to (S n) gs (Lam e) (Lam e')
+  | LetIn_erases_to n m gs e1 e2 e1' e2':
+    erases_to n gs e1 e1' ->
+    erases_to m (false :: gs) e2 e2' ->
+    erases_to  (S n + m) gs (LetIn e1 e2) (LetIn e1' e2')
+  | GRLetIn_erases_to n gs e1 e2 e2':
+    ghost_ok e1 ->
+    (∀ f, e1.[upn (length gs) f] = e1) →
+    erases_to n (true :: gs) e2 e2' ->
+    erases_to (S n) gs (GRLetIn e1 e2) e2'
+  | Seq_erases_to n m gs e1 e2 e1' e2':
+    erases_to n gs e1 e1' ->
+    erases_to m gs e2 e2' ->
+    erases_to (S n + m) gs (Seq e1 e2) (Seq e1' e2')
+  | GRSeq_erases_to n gs e1 e2 e2':
+    ghost_ok e1 ->
+    (∀ f, e1.[upn (length gs) f] = e1) →
+    erases_to n gs e2 e2' ->
+    erases_to (S n) gs (GRSeq e1 e2) e2'
+  | App_erases_to n m gs e1 e2 e1' e2':
+    erases_to n gs e1 e1' ->
+    erases_to m gs e2 e2' ->
+    erases_to (S n + m) gs (App e1 e2) (App e1' e2')
   | Unit_erases_to gs:
-    erases_to_core gs Unit Unit
+    erases_to 0 gs Unit Unit
   | Nat_erases_to gs n:
-    erases_to_core gs (Nat n) (Nat n)
+    erases_to 0 gs (Nat n) (Nat n)
   | Bool_erases_to gs b:
-    erases_to_core gs (Bool b) (Bool b)
-  | BinOp_erases_to gs op e1 e2 e1' e2':
-    erases_to gs e1 e1' ->
-    erases_to gs e2 e2' ->
-    erases_to_core gs (BinOp op e1 e2) (BinOp op e1' e2')
-  | If_erases_to gs e0 e1 e2 e0' e1' e2':
-    erases_to gs e0 e0' ->
-    erases_to gs e1 e1' ->
-    erases_to gs e2 e2' ->
-    erases_to_core gs (If e0 e1 e2) (If e0' e1' e2')
-  | Pair_erases_to gs e1 e2 e1' e2':
-    erases_to gs e1 e1' ->
-    erases_to gs e2 e2' ->
-    erases_to_core gs (Pair e1 e2) (Pair e1' e2')
-  | Fst_erases_to gs e e':
-    erases_to gs e e' ->
-    erases_to_core gs (Fst e) (Fst e')
-  | Snd_erases_to gs e e':
-    erases_to gs e e' ->
-    erases_to_core gs (Snd e) (Snd e')
-  | InjL_erases_to gs e e':
-    erases_to gs e e' ->
-    erases_to_core gs (InjL e) (InjL e')
-  | InjR_erases_to gs e e':
-    erases_to gs e e' ->
-    erases_to_core gs (InjR e) (InjR e')
-  | Case_erases_to gs e0 e1 e2 e0' e1' e2':
-    erases_to gs e0 e0' ->
-    erases_to (false :: gs) e1 e1' ->
-    erases_to (false :: gs) e2 e2' ->
-    erases_to_core gs (Case e0 e1 e2) (Case e0' e1' e2')
-  | Fold_erases_to gs e e':
-    erases_to gs e e' ->
-    erases_to_core gs (Fold e) (Fold e')
-  | Unfold_erases_to gs e e':
-    erases_to gs e e' ->
-    erases_to_core gs (Unfold e) (Unfold e')
-  | TLam_erases_to gs e e':
-    erases_to gs e e' ->
-    erases_to_core gs (TLam e) (TLam e')
-  | TApp_erases_to gs e e':
-    erases_to gs e e' ->
-    erases_to_core gs (TApp e) (TApp e')
-  | Fork_erases_to gs e e':
-    erases_to gs e e' ->
-    erases_to_core gs (Fork e) (Fork e')
+    erases_to 0 gs (Bool b) (Bool b)
+  | BinOp_erases_to n m gs op e1 e2 e1' e2':
+    erases_to n gs e1 e1' ->
+    erases_to m gs e2 e2' ->
+    erases_to (S n + m) gs (BinOp op e1 e2) (BinOp op e1' e2')
+  | If_erases_to n m k gs e0 e1 e2 e0' e1' e2':
+    erases_to n gs e0 e0' ->
+    erases_to m gs e1 e1' ->
+    erases_to k gs e2 e2' ->
+    erases_to (S n + m + k) gs (If e0 e1 e2) (If e0' e1' e2')
+  | Pair_erases_to n m gs e1 e2 e1' e2':
+    erases_to n gs e1 e1' ->
+    erases_to m gs e2 e2' ->
+    erases_to (S n + m) gs (Pair e1 e2) (Pair e1' e2')
+  | Fst_erases_to n gs e e':
+    erases_to n gs e e' ->
+    erases_to (S n) gs (Fst e) (Fst e')
+  | Snd_erases_to n gs e e':
+    erases_to n gs e e' ->
+    erases_to (S n) gs (Snd e) (Snd e')
+  | InjL_erases_to n gs e e':
+    erases_to n gs e e' ->
+    erases_to (S n) gs (InjL e) (InjL e')
+  | InjR_erases_to n gs e e':
+    erases_to n gs e e' ->
+    erases_to (S n) gs (InjR e) (InjR e')
+  | Case_erases_to n m k gs e0 e1 e2 e0' e1' e2':
+    erases_to n gs e0 e0' ->
+    erases_to m (false :: gs) e1 e1' ->
+    erases_to k (false :: gs) e2 e2' ->
+    erases_to (S n + m + k) gs (Case e0 e1 e2) (Case e0' e1' e2')
+  | Fold_erases_to n gs e e':
+    erases_to n gs e e' ->
+    erases_to (S n) gs (Fold e) (Fold e')
+  | Unfold_erases_to n gs e e':
+    erases_to n gs e e' ->
+    erases_to (S n) gs (Unfold e) (Unfold e')
+  | TLam_erases_to n gs e e':
+    erases_to n gs e e' ->
+    erases_to (S n) gs (TLam e) (TLam e')
+  | TApp_erases_to n gs e e':
+    erases_to n gs e e' ->
+    erases_to (S n) gs (TApp e) (TApp e')
+  | Fork_erases_to n gs e e':
+    erases_to n gs e e' ->
+    erases_to (S n) gs (Fork e) (Fork e')
   | Loc_erases_to gs l:
-    erases_to_core gs (Loc l) (Loc l)
+    erases_to 0 gs (Loc l) (Loc l)
   | IOtag_erases_to gs t:
-    erases_to_core gs (IOtag t) (IOtag t)
-  | Alloc_erases_to gs e e':
-    erases_to gs e e' ->
-    erases_to_core gs (Alloc e) (Alloc e')
-  | Load_erases_to gs e e':
-    erases_to gs e e' ->
-    erases_to_core gs (Load e) (Load e')
-  | Store_erases_to gs e1 e2 e1' e2':
-    erases_to gs e1 e1' ->
-    erases_to gs e2 e2' ->
-    erases_to_core gs (Store e1 e2) (Store e1' e2')
-  | CAS_erases_to gs e0 e1 e2 e0' e1' e2':
-    erases_to gs e0 e0' ->
-    erases_to gs e1 e1' ->
-    erases_to gs e2 e2' ->
-    erases_to_core gs (CAS e0 e1 e2) (CAS e0' e1' e2')
+    erases_to 0 gs (IOtag t) (IOtag t)
+  | Alloc_erases_to n gs e e':
+    erases_to n gs e e' ->
+    erases_to (S n) gs (Alloc e) (Alloc e')
+  | Load_erases_to n gs e e':
+    erases_to n gs e e' ->
+    erases_to (S n) gs (Load e) (Load e')
+  | Store_erases_to n m gs e1 e2 e1' e2':
+    erases_to n gs e1 e1' ->
+    erases_to m gs e2 e2' ->
+    erases_to (S n + m) gs (Store e1 e2) (Store e1' e2')
+  | CAS_erases_to n m k gs e0 e1 e2 e0' e1' e2':
+    erases_to n gs e0 e0' ->
+    erases_to m gs e1 e1' ->
+    erases_to k gs e2 e2' ->
+    erases_to (S n + m + k) gs (CAS e0 e1 e2) (CAS e0' e1' e2')
   | Rand_erases_to gs:
-    erases_to_core gs Rand Rand
-  | IO_erases_to gs e1 e2 e1' e2':
-    erases_to gs e1 e1' ->
-    erases_to gs e2 e2' ->
-    erases_to_core gs (IO e1 e2) (IO e1' e2')
-  with
-  erases_to : list bool -> expr -> expr -> Prop :=
-  | GRLetIn_erases_to gs e1 e2 e2':
-    ghost_ok e1 ->
-    erases_to (true :: gs) e2 e2' ->
-    erases_to gs (GRLetIn e1 e2) e2'
-  | GRSeq_erases_to gs e1 e2 e2':
-    ghost_ok e1 ->
-    erases_to gs e2 e2' ->
-    erases_to gs (GRSeq e1 e2) e2'
-  | erases_to_cong gs e e':
-      erases_to_core gs e e' -> erases_to gs e e'.
+    erases_to 0 gs Rand Rand
+  | IO_erases_to n m gs e1 e2 e1' e2':
+    erases_to n gs e1 e1' ->
+    erases_to m gs e2 e2' ->
+    erases_to (S n + m) gs (IO e1 e2) (IO e1' e2')
+  .
+
+  Lemma erases_to_closed n gb e e' f :
+    erases_to n gb e e' → e.[upn (length gb) f] = e.
+  Proof.
+    induction 1; eauto using var_erases_to_closed; asimpl in *;
+    repeat match goal with
+           | H : _ = _ :> expr |- _ => progress (rewrite H; clear H)
+           | H : forall _, _ = _ :> expr |- _ => progress (rewrite H; clear H)
+           end; auto.
+  Qed.
 
   Inductive val_erases_to: val -> val -> Prop :=
-  | RecV_erases_to e e':
-    erases_to (false :: false :: []) e e' ->
+  | RecV_erases_to n e e':
+    erases_to n (false :: false :: []) e e' ->
     val_erases_to (RecV e) (RecV e')
-  | LamV_erases_to e e':
-    erases_to (false :: []) e e' ->
+  | LamV_erases_to n e e':
+    erases_to n (false :: []) e e' ->
     val_erases_to (LamV e) (LamV e')
   | UnitV_erases_to:
     val_erases_to UnitV UnitV
@@ -168,37 +206,180 @@ Fixpoint ghost_ok(e: expr): Prop :=
   | FoldV_erases_to v v':
     val_erases_to v v' ->
     val_erases_to (FoldV v) (FoldV v')
-  | TLamV_erases_to e e':
-    erases_to [] e e' ->
+  | TLamV_erases_to n e e':
+    erases_to n [] e e' ->
     val_erases_to (TLamV e) (TLamV e')
   | LocV_erases_to l:
     val_erases_to (LocV l) (LocV l)
   | IOtagV_erases_to t:
     val_erases_to (IOtagV t) (IOtagV t).
 
+  Lemma upn_plus n m f : upn n (upn m f) = upn (n + m) f.
+  Proof.
+    revert f. induction m => f; asimpl; auto.
+    replace (upn (S m) f) with (upn m (up f)) by by asimpl.
+    by rewrite IHm; asimpl.
+  Qed.
+
+  Lemma closed_ren e k n m :
+    (∀ f : var → expr, e.[upn n f] = e) →
+    (∀ f : var → expr, e.[upn k (ren (+m))].[upn (m + n) f] = e.[upn k (ren (+m))]).
+  Proof.
+    revert k n m; induction e; intros k n' m He f.
+    - asimpl.
+      rewrite iter_up.
+      destruct lt_dec.
+      + asimpl.
+        rewrite iter_up.
+        destruct lt_dec; auto.
+        specialize (He (λ _, Unit)); asimpl in *.
+        rewrite iter_up in He.
+        destruct lt_dec; by try omega.
+      + asimpl.
+        rewrite iter_up.
+        destruct lt_dec; auto.
+        specialize (He (λ _, Unit)); asimpl in *.
+        rewrite iter_up in He.
+        destruct lt_dec; by try omega.
+    - assert (∀ f : var → expr, e.[upn (2 + n') f] = e) as He'.
+      { intros f'; specialize (He f'); asimpl in *; by simplify_eq. }
+      specialize (IHe (2 + k) (2 + n') m He' f).
+      asimpl; rewrite upn_plus; erewrite <- IHe; asimpl; eauto.
+    - assert (∀ f : var → expr, e.[upn (1 + n') f] = e) as He'.
+      { intros f'; specialize (He f'); asimpl in *; by simplify_eq. }
+      specialize (IHe (1 + k) (1 + n') m He' f).
+      simpl in *.
+      asimpl. erewrite <- IHe; asimpl; eauto.
+    - asimpl. admit.
+  Admitted.
+
+  Lemma subst_closed e e' n m:
+    (∀ f : var → expr, e.[upn (S n + m) f] = e) →
+    (∀ f : var → expr, e'.[upn m f] = e') →
+    ∀ f : var → expr, e.[upn n (e' .: ids)].[upn (n + m) f] = e.[upn n (e' .: ids)].
+  Proof.
+    revert n m e'; induction e; intros n' m e' He He' f.
+    - asimpl.
+      unfold var in *.
+      rewrite iter_up; destruct lt_dec.
+      + asimpl. rewrite iter_up. destruct lt_dec; try omega; auto.
+      + asimpl.
+        destruct (x - n') eqn:Heqx.
+        * asimpl in *.
+          transitivity e'.[ren (+n')].[upn (n' + m) f]; first by asimpl.
+          eapply (closed_ren _ 0); eauto.
+        * asimpl.
+          rewrite iter_up; destruct lt_dec; auto.
+          specialize (He (λ _, Unit)).
+          asimpl in *.
+          rewrite iter_up in He.
+          destruct lt_dec; by try omega.
+    - asimpl.
+      assert (∀ f : var → expr, e.[upn (3 + n' + m) f] = e) as He''.
+      { intros f'; specialize (He f'); asimpl in *; by simplify_eq. }
+      specialize (IHe (2 + n') m e' He'' He' f).
+      asimpl; rewrite upn_plus; erewrite <- IHe; asimpl; eauto.
+  Admitted.
+
+  Lemma erases_to_subst gs gs' n e e' e'':
+    erases_to n (gs ++ true :: gs') e e' →
+    ghost_ok e'' →
+    (forall f, e''.[upn (length gs') f] = e'') →
+    erases_to n (gs ++ gs') e.[upn (length gs) (e'' .: ids)] e'.
+  Proof.
+    remember (gs ++ true :: gs') as GS.
+    intros Her.
+    revert gs gs' HeqGS.
+    induction Her; intros gs1 gs2 HeqGS Hgok He''cl; subst; asimpl;
+      try by (constructor; try apply (IHHer (_ :: _));
+           try apply (IHHer (_ :: _ :: _));
+           try apply (IHHer2 (_ :: _));
+           try apply (IHHer3 (_ :: _)); eauto).
+    - clear He''cl.
+      rewrite iter_up.
+      destruct lt_dec as [Hlt|Hn].
+      + constructor.
+        revert x x' H Hlt.
+        induction gs1; intros x x' H Hlt; simpl in *; first omega.
+        destruct x; inversion H; simplify_eq.
+        * constructor.
+        * constructor. apply IHgs1; eauto with omega.
+        * constructor. apply IHgs1; eauto with omega.
+      + destruct (decide (x = length gs1)); subst.
+        * apply var_erases_to_not_ghost in H.
+          rewrite lookup_app_r in H; auto with omega.
+          replace (length gs1 - length gs1) with 0 in H by omega.
+          done.
+        * unfold var in *.
+          destruct (x - length gs1) eqn:Heqx; first omega.
+          asimpl.
+          constructor.
+          replace (length gs1 + n0) with (pred x) by omega.
+          assert (length gs1 < x) as Hgt by omega.
+          clear -Hgt H.
+          revert x x' gs2 H Hgt.
+          induction gs1; intros x x' gs2 H Hgt; simpl in *.
+          -- by inversion H; subst; simpl.
+          -- inversion H; simplify_eq; try omega.
+             ++ replace ((pred (S x0))) with (S (pred x0)) by omega.
+                constructor; auto with omega.
+             ++ replace ((pred (S x0))) with (S (pred x0)) by omega.
+                constructor; auto with omega.
+    - constructor.
+      + apply ghost_ok_subst; auto.
+        intros x.
+        rewrite iter_up; destruct lt_dec; simpl; auto.
+        asimpl. destruct (x - length gs1) eqn:Heqx.
+        asimpl.
+        by apply ghost_ok_subst; eauto; asimpl.
+        by asimpl.
+      + intros f.
+        rewrite app_length.
+        apply subst_closed; auto.
+        revert H0. rewrite app_length /=.
+        by replace (length gs1 + S (length gs2)) with (S (length gs1) + (length gs2))
+          by omega.
+      + apply (IHHer (_ :: _)); eauto.
+    - constructor.
+      + apply ghost_ok_subst; auto.
+        intros x.
+        rewrite iter_up; destruct lt_dec; simpl; auto.
+        asimpl. destruct (x - length gs1) eqn:Heqx.
+        asimpl.
+        by apply ghost_ok_subst; eauto; asimpl.
+        by asimpl.
+      + intros f.
+        rewrite app_length.
+        apply subst_closed; auto.
+        revert H0. rewrite app_length /=.
+        by replace (length gs1 + S (length gs2)) with (S (length gs1) + (length gs2))
+          by omega.
+      + apply (IHHer _); eauto.
+  Qed.
+
   Inductive ectx_item_erases_to: ectx_item -> ectx_item -> Prop :=
-  | AppLCtx_erases_to e e' :
-      erases_to [] e e' →
+  | AppLCtx_erases_to n e e' :
+      erases_to n [] e e' →
       ectx_item_erases_to (AppLCtx e) (AppLCtx e')
   | AppRCtx_erases_to v v' :
       val_erases_to v v' →
       ectx_item_erases_to (AppRCtx v) (AppRCtx v')
-  | LetInCtx_erases_to e e' :
-      erases_to [] e e' →
+  | LetInCtx_erases_to n e e' :
+      erases_to n [false] e e' →
       ectx_item_erases_to (LetInCtx e) (LetInCtx e')
-  | SeqCtx_erases_to e e' :
-      erases_to [] e e' →
+  | SeqCtx_erases_to n e e' :
+      erases_to n [] e e' →
       ectx_item_erases_to (SeqCtx e) (SeqCtx e')
   | TAppCtx_erases_to :
       ectx_item_erases_to TAppCtx TAppCtx
-  | PairLCtx_erases_to e e' :
-      erases_to [] e e' →
+  | PairLCtx_erases_to n e e' :
+      erases_to n [] e e' →
       ectx_item_erases_to (PairLCtx e) (PairLCtx e')
   | PairRCtx_erases_to v v' :
       val_erases_to v v' →
       ectx_item_erases_to (PairRCtx v) (PairRCtx v')
-  | BinOpLCtx_erases_to op e e' :
-      erases_to [] e e' →
+  | BinOpLCtx_erases_to n op e e' :
+      erases_to n [] e e' →
       ectx_item_erases_to (BinOpLCtx op e) (BinOpLCtx op e')
   | BinOpRCtx_erases_to op v v' :
       val_erases_to v v' →
@@ -211,13 +392,13 @@ Fixpoint ghost_ok(e: expr): Prop :=
       ectx_item_erases_to InjLCtx InjLCtx
   | InjRCtx_erases_to :
       ectx_item_erases_to InjRCtx InjRCtx
-  | CaseCtx_erases_to e1 e1' e2 e2' :
-      erases_to (false :: []) e1 e1' →
-      erases_to (false :: []) e2 e2' →
+  | CaseCtx_erases_to n m e1 e1' e2 e2' :
+      erases_to n (false :: []) e1 e1' →
+      erases_to m (false :: []) e2 e2' →
       ectx_item_erases_to (CaseCtx e1 e2) (CaseCtx e1' e2')
-  | IfCtx_erases_to e1 e1' e2 e2' :
-      erases_to [] e1 e1' →
-      erases_to [] e2 e2' →
+  | IfCtx_erases_to n m e1 e1' e2 e2' :
+      erases_to n [] e1 e1' →
+      erases_to m [] e2 e2' →
       ectx_item_erases_to (IfCtx e1 e2) (IfCtx e1' e2')
   | FoldCtx_erases_to :
       ectx_item_erases_to FoldCtx FoldCtx
@@ -227,26 +408,26 @@ Fixpoint ghost_ok(e: expr): Prop :=
       ectx_item_erases_to AllocCtx AllocCtx
   | LoadCtx_erases_to :
       ectx_item_erases_to LoadCtx LoadCtx
-  | StoreLCtx_erases_to e e' :
-      erases_to [] e e' →
+  | StoreLCtx_erases_to n e e' :
+      erases_to n [] e e' →
       ectx_item_erases_to (StoreLCtx e) (StoreLCtx e')
   | StoreRCtx_erases_to v v' :
       val_erases_to v v' →
       ectx_item_erases_to (StoreRCtx v) (StoreRCtx v')
-  | CasLCtx_erases_to e2 e2' e3 e3' :
-      erases_to [] e2 e2' →
-      erases_to [] e3 e3' →
+  | CasLCtx_erases_to n m e2 e2' e3 e3' :
+      erases_to n [] e2 e2' →
+      erases_to m [] e3 e3' →
       ectx_item_erases_to (CasLCtx e2 e3) (CasLCtx e2' e3')
-  | CasMCtx_erases_to v1 v1' e3 e3' :
+  | CasMCtx_erases_to n v1 v1' e3 e3' :
       val_erases_to v1 v1' →
-      erases_to [] e3 e3' →
+      erases_to n [] e3 e3' →
       ectx_item_erases_to (CasMCtx v1 e3) (CasMCtx v1' e3')
   | CasRCtx_erases_to v1 v1' v2 v2' :
       val_erases_to v1 v1' →
       val_erases_to v2 v2' →
       ectx_item_erases_to (CasRCtx v1 v2) (CasRCtx v1' v2')
-  | IOLCtx_erases_to e e' :
-      erases_to [] e e' →
+  | IOLCtx_erases_to n e e' :
+      erases_to n [] e e' →
       ectx_item_erases_to (IOLCtx e) (IOLCtx e')
   | IORCtx_erases_to v v' :
       val_erases_to v v' →
